<?xml version="1.0"?>


<!DOCTYPE rdf:RDF [
    <!ENTITY owl "http://www.w3.org/2002/07/owl#" >
    <!ENTITY xsd "http://www.w3.org/2001/XMLSchema#" >
    <!ENTITY rdfs "http://www.w3.org/2000/01/rdf-schema#" >
    <!ENTITY rdf "http://www.w3.org/1999/02/22-rdf-syntax-ns#" >
]>


<rdf:RDF xmlns="http://se-on.org/ontologies/domain-specific/2012/02/history.owl#"
     xml:base="http://se-on.org/ontologies/domain-specific/2012/02/history.owl"
     xmlns:rdfs="http://www.w3.org/2000/01/rdf-schema#"
     xmlns:owl="http://www.w3.org/2002/07/owl#"
     xmlns:xsd="http://www.w3.org/2001/XMLSchema#"
     xmlns:rdf="http://www.w3.org/1999/02/22-rdf-syntax-ns#">
    <owl:Ontology rdf:about="http://se-on.org/ontologies/domain-specific/2012/02/history.owl">
        <rdfs:comment>This ontology is part of SEON. It defines concepts to describe the history of files managed by version control system.</rdfs:comment>
        <owl:imports rdf:resource="http://se-on.org/ontologies/general/2012/02/main.owl"/>
    </owl:Ontology>
    


    <!-- 
    ///////////////////////////////////////////////////////////////////////////////////////
    //
    // Annotation properties
    //
    ///////////////////////////////////////////////////////////////////////////////////////
     -->

    


    <!-- 
    ///////////////////////////////////////////////////////////////////////////////////////
    //
    // Datatypes
    //
    ///////////////////////////////////////////////////////////////////////////////////////
     -->

    


    <!-- 
    ///////////////////////////////////////////////////////////////////////////////////////
    //
    // Object Properties
    //
    ///////////////////////////////////////////////////////////////////////////////////////
     -->

    


    <!-- http://se-on.org/ontologies/domain-specific/2012/02/history.owl#appearsInRelease -->

    <owl:ObjectProperty rdf:about="http://se-on.org/ontologies/domain-specific/2012/02/history.owl#appearsInRelease">
        <rdfs:comment>A certain version of a file can be chosen for a release.</rdfs:comment>
        <rdfs:domain rdf:resource="http://se-on.org/ontologies/domain-specific/2012/02/history.owl#Version"/>
        <rdfs:range rdf:resource="http://se-on.org/ontologies/general/2012/02/main.owl#Release"/>
    </owl:ObjectProperty>
    


    <!-- http://se-on.org/ontologies/domain-specific/2012/02/history.owl#commitsChangeSet -->

    <owl:ObjectProperty rdf:about="http://se-on.org/ontologies/domain-specific/2012/02/history.owl#commitsChangeSet">
        <rdfs:comment>Committers submit a set of changed files to a version control system. This property relates the committer to the change set.</rdfs:comment>
        <rdfs:range rdf:resource="http://se-on.org/ontologies/domain-specific/2012/02/history.owl#ChangeSet"/>
        <rdfs:domain rdf:resource="http://se-on.org/ontologies/domain-specific/2012/02/history.owl#Committer"/>
        <owl:propertyChainAxiom rdf:parseType="Collection">
            <rdf:Description rdf:about="http://se-on.org/ontologies/domain-specific/2012/02/history.owl#commitsVersion"/>
            <rdf:Description rdf:about="http://se-on.org/ontologies/domain-specific/2012/02/history.owl#isCommittedIn"/>
        </owl:propertyChainAxiom>
    </owl:ObjectProperty>
    


    <!-- http://se-on.org/ontologies/domain-specific/2012/02/history.owl#commitsVersion -->

    <owl:ObjectProperty rdf:about="http://se-on.org/ontologies/domain-specific/2012/02/history.owl#commitsVersion">
        <rdfs:comment>A committer submits a particular version of a file per commit to a version control system. This property relates the comitter to such a version.</rdfs:comment>
        <rdfs:domain rdf:resource="http://se-on.org/ontologies/domain-specific/2012/02/history.owl#Committer"/>
        <rdfs:range rdf:resource="http://se-on.org/ontologies/domain-specific/2012/02/history.owl#Version"/>
        <owl:inverseOf rdf:resource="http://se-on.org/ontologies/domain-specific/2012/02/history.owl#isCommittedBy"/>
    </owl:ObjectProperty>
    


    <!-- http://se-on.org/ontologies/domain-specific/2012/02/history.owl#constituesVersion -->

    <owl:ObjectProperty rdf:about="http://se-on.org/ontologies/domain-specific/2012/02/history.owl#constituesVersion">
        <rdfs:comment>A commit will lead to a new version of a file. This is denoted by this property.</rdfs:comment>
        <rdfs:domain rdf:resource="http://se-on.org/ontologies/domain-specific/2012/02/history.owl#Commit"/>
        <rdfs:range rdf:resource="http://se-on.org/ontologies/domain-specific/2012/02/history.owl#Version"/>
    </owl:ObjectProperty>
    


    <!-- http://se-on.org/ontologies/domain-specific/2012/02/history.owl#containsVersion -->

    <owl:ObjectProperty rdf:about="http://se-on.org/ontologies/domain-specific/2012/02/history.owl#containsVersion">
        <rdfs:comment>Change sets contain one or more files with a particular version each.</rdfs:comment>
        <rdfs:domain rdf:resource="http://se-on.org/ontologies/domain-specific/2012/02/history.owl#ChangeSet"/>
        <rdfs:range rdf:resource="http://se-on.org/ontologies/domain-specific/2012/02/history.owl#Version"/>
    </owl:ObjectProperty>
    


    <!-- http://se-on.org/ontologies/domain-specific/2012/02/history.owl#followsVersion -->

    <owl:ObjectProperty rdf:about="http://se-on.org/ontologies/domain-specific/2012/02/history.owl#followsVersion">
        <rdfs:comment>A version, if not the first one in the history, always follows an earlier one.</rdfs:comment>
        <rdfs:range rdf:resource="http://se-on.org/ontologies/domain-specific/2012/02/history.owl#Version"/>
        <rdfs:domain rdf:resource="http://se-on.org/ontologies/domain-specific/2012/02/history.owl#Version"/>
        <owl:inverseOf rdf:resource="http://se-on.org/ontologies/domain-specific/2012/02/history.owl#precedesVersion"/>
    </owl:ObjectProperty>
    


    <!-- http://se-on.org/ontologies/domain-specific/2012/02/history.owl#hasVersion -->

    <owl:ObjectProperty rdf:about="http://se-on.org/ontologies/domain-specific/2012/02/history.owl#hasVersion">
        <rdfs:comment>A file can exist in several versions.</rdfs:comment>
        <rdfs:domain rdf:resource="http://se-on.org/ontologies/domain-specific/2012/02/history.owl#FileUnderVersionControl"/>
        <rdfs:range rdf:resource="http://se-on.org/ontologies/domain-specific/2012/02/history.owl#Version"/>
    </owl:ObjectProperty>
    


    <!-- http://se-on.org/ontologies/domain-specific/2012/02/history.owl#isCommittedBy -->

    <owl:ObjectProperty rdf:about="http://se-on.org/ontologies/domain-specific/2012/02/history.owl#isCommittedBy">
        <rdfs:comment>A version of a file can be committed to a version control system by a committer.</rdfs:comment>
        <rdfs:range rdf:resource="http://se-on.org/ontologies/domain-specific/2012/02/history.owl#Committer"/>
        <rdfs:domain rdf:resource="http://se-on.org/ontologies/domain-specific/2012/02/history.owl#Version"/>
    </owl:ObjectProperty>
    


    <!-- http://se-on.org/ontologies/domain-specific/2012/02/history.owl#isCommittedIn -->

    <owl:ObjectProperty rdf:about="http://se-on.org/ontologies/domain-specific/2012/02/history.owl#isCommittedIn">
        <rdfs:comment>A version of a file is committed in a change set to a version control system.</rdfs:comment>
        <rdfs:range rdf:resource="http://se-on.org/ontologies/domain-specific/2012/02/history.owl#ChangeSet"/>
        <rdfs:domain rdf:resource="http://se-on.org/ontologies/domain-specific/2012/02/history.owl#Version"/>
        <owl:inverseOf rdf:resource="http://se-on.org/ontologies/domain-specific/2012/02/history.owl#containsVersion"/>
    </owl:ObjectProperty>
    


    <!-- http://se-on.org/ontologies/domain-specific/2012/02/history.owl#isOnBranch -->

    <owl:ObjectProperty rdf:about="http://se-on.org/ontologies/domain-specific/2012/02/history.owl#isOnBranch">
        <rdfs:comment>Particular versions of a file can be on a separate development stream, i.e., a branch.</rdfs:comment>
        <rdfs:range rdf:resource="http://se-on.org/ontologies/domain-specific/2012/02/history.owl#Branch"/>
        <rdfs:domain rdf:resource="http://se-on.org/ontologies/domain-specific/2012/02/history.owl#Version"/>
    </owl:ObjectProperty>
    


    <!-- http://se-on.org/ontologies/domain-specific/2012/02/history.owl#isVersionOf -->

    <owl:ObjectProperty rdf:about="http://se-on.org/ontologies/domain-specific/2012/02/history.owl#isVersionOf">
        <rdfs:comment>A version belongs to a particular file managed by a version control system.</rdfs:comment>
        <rdfs:range rdf:resource="http://se-on.org/ontologies/domain-specific/2012/02/history.owl#FileUnderVersionControl"/>
        <rdfs:domain rdf:resource="http://se-on.org/ontologies/domain-specific/2012/02/history.owl#Version"/>
        <owl:inverseOf rdf:resource="http://se-on.org/ontologies/domain-specific/2012/02/history.owl#hasVersion"/>
    </owl:ObjectProperty>
    


    <!-- http://se-on.org/ontologies/domain-specific/2012/02/history.owl#performsCommit -->

    <owl:ObjectProperty rdf:about="http://se-on.org/ontologies/domain-specific/2012/02/history.owl#performsCommit">
        <rdfs:comment>A committer performs a commit when he submits new versions of files to a version control system.</rdfs:comment>
        <rdfs:range rdf:resource="http://se-on.org/ontologies/domain-specific/2012/02/history.owl#Commit"/>
        <rdfs:domain rdf:resource="http://se-on.org/ontologies/domain-specific/2012/02/history.owl#Committer"/>
    </owl:ObjectProperty>
    


    <!-- http://se-on.org/ontologies/domain-specific/2012/02/history.owl#precedesVersion -->

    <owl:ObjectProperty rdf:about="http://se-on.org/ontologies/domain-specific/2012/02/history.owl#precedesVersion">
        <rdfs:comment>A version, if not the last one in the history, always precedes an later one.</rdfs:comment>
        <rdfs:range rdf:resource="http://se-on.org/ontologies/domain-specific/2012/02/history.owl#Version"/>
        <rdfs:domain rdf:resource="http://se-on.org/ontologies/domain-specific/2012/02/history.owl#Version"/>
    </owl:ObjectProperty>
    


    <!-- 
    ///////////////////////////////////////////////////////////////////////////////////////
    //
    // Data properties
    //
    ///////////////////////////////////////////////////////////////////////////////////////
     -->

    


    <!-- http://se-on.org/ontologies/domain-specific/2012/02/history.owl#committedOn -->

    <owl:DatatypeProperty rdf:about="http://se-on.org/ontologies/domain-specific/2012/02/history.owl#committedOn">
        <rdfs:comment>Change sets or versions are committed at a particular point in time.</rdfs:comment>
        <rdfs:subPropertyOf rdf:resource="http://se-on.org/ontologies/general/2012/2/main.owl#hasCreationDate"/>
        <rdfs:domain>
            <owl:Class>
                <owl:unionOf rdf:parseType="Collection">
                    <rdf:Description rdf:about="http://se-on.org/ontologies/domain-specific/2012/02/history.owl#ChangeSet"/>
                    <rdf:Description rdf:about="http://se-on.org/ontologies/domain-specific/2012/02/history.owl#Version"/>
                </owl:unionOf>
            </owl:Class>
        </rdfs:domain>
    </owl:DatatypeProperty>
    


    <!-- http://se-on.org/ontologies/domain-specific/2012/02/history.owl#hasCommitMessage -->

    <owl:DatatypeProperty rdf:about="http://se-on.org/ontologies/domain-specific/2012/02/history.owl#hasCommitMessage">
        <rdfs:comment>A change set or single version have a commit message denoting the reason for the change.</rdfs:comment>
        <rdfs:range rdf:resource="&xsd;string"/>
        <rdfs:domain>
            <owl:Class>
                <owl:unionOf rdf:parseType="Collection">
                    <rdf:Description rdf:about="http://se-on.org/ontologies/domain-specific/2012/02/history.owl#ChangeSet"/>
                    <rdf:Description rdf:about="http://se-on.org/ontologies/domain-specific/2012/02/history.owl#Version"/>
                </owl:unionOf>
            </owl:Class>
        </rdfs:domain>
    </owl:DatatypeProperty>
    


    <!-- http://se-on.org/ontologies/domain-specific/2012/02/history.owl#hasContentIdentifier -->

    <owl:DatatypeProperty rdf:about="http://se-on.org/ontologies/domain-specific/2012/02/history.owl#hasContentIdentifier">
        <rdfs:comment>A version of a file is denoted by a number, hash value, etc.</rdfs:comment>
        <rdfs:domain rdf:resource="http://se-on.org/ontologies/domain-specific/2012/02/history.owl#Version"/>
        <rdfs:subPropertyOf rdf:resource="http://se-on.org/ontologies/general/2012/02/main.owl#hasIdentifier"/>
        <rdfs:range rdf:resource="&rdfs;Literal"/>
    </owl:DatatypeProperty>
    


    <!-- http://se-on.org/ontologies/domain-specific/2012/02/history.owl#hasTag -->

    <owl:DatatypeProperty rdf:about="http://se-on.org/ontologies/domain-specific/2012/02/history.owl#hasTag">
        <rdfs:comment>Branches or releases can be tagged.</rdfs:comment>
        <rdfs:range rdf:resource="&xsd;string"/>
        <rdfs:domain>
            <owl:Class>
                <owl:unionOf rdf:parseType="Collection">
                    <rdf:Description rdf:about="http://se-on.org/ontologies/domain-specific/2012/02/history.owl#Branch"/>
                    <rdf:Description rdf:about="http://se-on.org/ontologies/general/2012/02/main.owl#Release"/>
                </owl:unionOf>
            </owl:Class>
        </rdfs:domain>
    </owl:DatatypeProperty>
    


    <!-- http://se-on.org/ontologies/domain-specific/2012/02/history.owl#linesAdded -->

    <owl:DatatypeProperty rdf:about="http://se-on.org/ontologies/domain-specific/2012/02/history.owl#linesAdded">
        <rdfs:domain rdf:resource="http://se-on.org/ontologies/domain-specific/2012/02/history.owl#Version"/>
        <rdfs:range rdf:resource="&xsd;int"/>
        <rdfs:subPropertyOf rdf:resource="&owl;topDataProperty"/>
    </owl:DatatypeProperty>
    


    <!-- http://se-on.org/ontologies/domain-specific/2012/02/history.owl#linesDeleted -->

    <owl:DatatypeProperty rdf:about="http://se-on.org/ontologies/domain-specific/2012/02/history.owl#linesDeleted">
        <rdfs:domain rdf:resource="http://se-on.org/ontologies/domain-specific/2012/02/history.owl#Version"/>
        <rdfs:range rdf:resource="&xsd;int"/>
    </owl:DatatypeProperty>
    


    <!-- 
    ///////////////////////////////////////////////////////////////////////////////////////
    //
    // Classes
    //
    ///////////////////////////////////////////////////////////////////////////////////////
     -->

    


    <!-- http://se-on.org/ontologies/domain-specific/2012/02/history.owl#Branch -->

    <owl:Class rdf:about="http://se-on.org/ontologies/domain-specific/2012/02/history.owl#Branch">
        <rdfs:subClassOf rdf:resource="http://se-on.org/ontologies/general/2012/2/main.owl#SeonThing"/>
        <rdfs:comment>A separate development stream.</rdfs:comment>
    </owl:Class>
    


    <!-- http://se-on.org/ontologies/domain-specific/2012/02/history.owl#ChangeSet -->

    <owl:Class rdf:about="http://se-on.org/ontologies/domain-specific/2012/02/history.owl#ChangeSet">
        <rdfs:subClassOf rdf:resource="http://se-on.org/ontologies/general/2012/2/main.owl#SeonThing"/>
        <rdfs:comment>A set of files that change together, i.e., that were committet to a version control system together.</rdfs:comment>
    </owl:Class>
    


    <!-- http://se-on.org/ontologies/domain-specific/2012/02/history.owl#Commit -->

    <owl:Class rdf:about="http://se-on.org/ontologies/domain-specific/2012/02/history.owl#Commit">
        <rdfs:subClassOf rdf:resource="http://se-on.org/ontologies/general/2012/2/main.owl#Activity"/>
        <rdfs:comment>The act of committing changes to a version control system.</rdfs:comment>
    </owl:Class>
    


    <!-- http://se-on.org/ontologies/domain-specific/2012/02/history.owl#Committer -->

    <owl:Class rdf:about="http://se-on.org/ontologies/domain-specific/2012/02/history.owl#Committer">
        <rdfs:subClassOf rdf:resource="http://se-on.org/ontologies/general/2012/02/main.owl#Developer"/>
        <rdfs:comment>A developer that is allowed to commit changes to a version control system.</rdfs:comment>
    </owl:Class>
    


    <!-- http://se-on.org/ontologies/domain-specific/2012/02/history.owl#FileUnderVersionControl -->

    <owl:Class rdf:about="http://se-on.org/ontologies/domain-specific/2012/02/history.owl#FileUnderVersionControl">
        <rdfs:subClassOf rdf:resource="http://se-on.org/ontologies/general/2012/2/main.owl#File"/>
        <rdfs:comment>A file which is managed by a version control system.</rdfs:comment>
    </owl:Class>
    


    <!-- http://se-on.org/ontologies/domain-specific/2012/02/history.owl#Version -->

    <owl:Class rdf:about="http://se-on.org/ontologies/domain-specific/2012/02/history.owl#Version">
        <rdfs:subClassOf rdf:resource="http://se-on.org/ontologies/general/2012/2/main.owl#SeonThing"/>
        <rdfs:comment>A version of a file.</rdfs:comment>
    </owl:Class>
</rdf:RDF>



<!-- Generated by the OWL API (version 3.3.1957) http://owlapi.sourceforge.net -->

