<?xml version="1.0"?>


<!DOCTYPE rdf:RDF [
    <!ENTITY owl "http://www.w3.org/2002/07/owl#" >
    <!ENTITY xsd "http://www.w3.org/2001/XMLSchema#" >
    <!ENTITY rdfs "http://www.w3.org/2000/01/rdf-schema#" >
    <!ENTITY rdf "http://www.w3.org/1999/02/22-rdf-syntax-ns#" >
]>


<rdf:RDF xmlns="http://se-on.org/ontologies/domain-spanning/2012/02/change-couplings.owl#"
     xml:base="http://se-on.org/ontologies/domain-spanning/2012/02/change-couplings.owl"
     xmlns:rdfs="http://www.w3.org/2000/01/rdf-schema#"
     xmlns:owl="http://www.w3.org/2002/07/owl#"
     xmlns:xsd="http://www.w3.org/2001/XMLSchema#"
     xmlns:rdf="http://www.w3.org/1999/02/22-rdf-syntax-ns#">
    <owl:Ontology rdf:about="http://se-on.org/ontologies/domain-spanning/2012/02/change-couplings.owl">
        <owl:imports rdf:resource="http://se-on.org/ontologies/domain-specific/2012/02/history.owl"/>
    </owl:Ontology>
    


    <!-- 
    ///////////////////////////////////////////////////////////////////////////////////////
    //
    // Annotation properties
    //
    ///////////////////////////////////////////////////////////////////////////////////////
     -->

    


    <!-- 
    ///////////////////////////////////////////////////////////////////////////////////////
    //
    // Datatypes
    //
    ///////////////////////////////////////////////////////////////////////////////////////
     -->

    


    <!-- 
    ///////////////////////////////////////////////////////////////////////////////////////
    //
    // Object Properties
    //
    ///////////////////////////////////////////////////////////////////////////////////////
     -->

    


    <!-- http://se-on.org/ontologies/domain-spanning/2012/02/change-couplings.owl#belongsToCouplingClass -->

    <owl:ObjectProperty rdf:about="http://se-on.org/ontologies/domain-spanning/2012/02/change-couplings.owl#belongsToCouplingClass">
        <rdfs:comment>An artifact can belong to a class of coupled artifacts.</rdfs:comment>
        <rdfs:range rdf:resource="http://se-on.org/ontologies/domain-spanning/2012/02/change-couplings.owl#CouplingClass"/>
        <rdfs:domain rdf:resource="http://se-on.org/ontologies/general/2012/2/main.owl#Artifact"/>
        <rdfs:subPropertyOf rdf:resource="http://se-on.org/ontologies/general/2012/2/main.owl#hasParent"/>
    </owl:ObjectProperty>
    


    <!-- http://se-on.org/ontologies/domain-spanning/2012/02/change-couplings.owl#hasTypeOfCoupling -->

    <owl:ObjectProperty rdf:about="http://se-on.org/ontologies/domain-spanning/2012/02/change-couplings.owl#hasTypeOfCoupling">
        <rdfs:comment>A coupling class can have a type. For example, the class can contain logically coupled files, or Java classes that are coupled due to static source code dependencies.</rdfs:comment>
        <rdfs:domain rdf:resource="http://se-on.org/ontologies/domain-spanning/2012/02/change-couplings.owl#CouplingClass"/>
        <rdfs:range rdf:resource="http://se-on.org/ontologies/domain-spanning/2012/02/change-couplings.owl#TypeOfCoupling"/>
    </owl:ObjectProperty>
    


    <!-- http://se-on.org/ontologies/domain-spanning/2012/02/change-couplings.owl#isBasedOnChangeSet -->

    <owl:ObjectProperty rdf:about="http://se-on.org/ontologies/domain-spanning/2012/02/change-couplings.owl#isBasedOnChangeSet">
        <rdfs:comment>When files are changed together often, then they are logically coupled.</rdfs:comment>
        <rdfs:domain rdf:resource="http://se-on.org/ontologies/domain-spanning/2012/02/change-couplings.owl#CouplingClass"/>
        <rdfs:range rdf:resource="http://se-on.org/ontologies/domain-specific/2012/02/history.owl#ChangeSet"/>
    </owl:ObjectProperty>
    


    <!-- http://se-on.org/ontologies/domain-spanning/2012/02/change-couplings.owl#isCoupledWith -->

    <owl:ObjectProperty rdf:about="http://se-on.org/ontologies/domain-spanning/2012/02/change-couplings.owl#isCoupledWith">
        <rdf:type rdf:resource="&owl;SymmetricProperty"/>
        <rdfs:comment>Denotes that two artifacts are coupled with each other. In principle, coupling is a kind of dependency. However, the direction of the dependency relationship is unclear. For example, Artifact A and B could both depend on a business rule, leading to common commits. Because of this, it is not a subproperty of dependsOn.</rdfs:comment>
        <rdfs:range rdf:resource="http://se-on.org/ontologies/general/2012/2/main.owl#Artifact"/>
        <rdfs:domain rdf:resource="http://se-on.org/ontologies/general/2012/2/main.owl#Artifact"/>
    </owl:ObjectProperty>
    


    <!-- 
    ///////////////////////////////////////////////////////////////////////////////////////
    //
    // Classes
    //
    ///////////////////////////////////////////////////////////////////////////////////////
     -->

    


    <!-- http://se-on.org/ontologies/domain-spanning/2012/02/change-couplings.owl#CouplingClass -->

    <owl:Class rdf:about="http://se-on.org/ontologies/domain-spanning/2012/02/change-couplings.owl#CouplingClass">
        <rdfs:subClassOf rdf:resource="http://se-on.org/ontologies/general/2012/2/main.owl#SeonThing"/>
        <rdfs:comment>A class of files that are coupled with each others, e.g., because they often change together.</rdfs:comment>
    </owl:Class>
    


    <!-- http://se-on.org/ontologies/domain-spanning/2012/02/change-couplings.owl#TypeOfCoupling -->

    <owl:Class rdf:about="http://se-on.org/ontologies/domain-spanning/2012/02/change-couplings.owl#TypeOfCoupling">
        <rdfs:subClassOf rdf:resource="http://se-on.org/ontologies/general/2012/2/main.owl#SeonThing"/>
        <rdfs:comment>The nature of the coupling relation.</rdfs:comment>
    </owl:Class>
    


    <!-- 
    ///////////////////////////////////////////////////////////////////////////////////////
    //
    // Individuals
    //
    ///////////////////////////////////////////////////////////////////////////////////////
     -->

    


    <!-- http://se-on.org/ontologies/domain-spanning/2012/02/change-couplings.owl#logicalCoupling -->

    <owl:NamedIndividual rdf:about="http://se-on.org/ontologies/domain-spanning/2012/02/change-couplings.owl#logicalCoupling">
        <rdf:type rdf:resource="http://se-on.org/ontologies/domain-spanning/2012/02/change-couplings.owl#TypeOfCoupling"/>
    </owl:NamedIndividual>
    


    <!-- http://se-on.org/ontologies/domain-spanning/2012/02/change-couplings.owl#staticalCoupling -->

    <owl:NamedIndividual rdf:about="http://se-on.org/ontologies/domain-spanning/2012/02/change-couplings.owl#staticalCoupling">
        <rdf:type rdf:resource="http://se-on.org/ontologies/domain-spanning/2012/02/change-couplings.owl#TypeOfCoupling"/>
    </owl:NamedIndividual>
</rdf:RDF>



<!-- Generated by the OWL API (version 3.2.5.1912) http://owlapi.sourceforge.net -->

